theories/Shared/Libs/DLW/Vec/vec.v
@@ -162,20 +162,6 @@ Section vector.
     + repeat rewrite vec_change_neq; auto.
   Qed.
 
-  Lemma vec_change_comm n v p q x y : p <> q ->
-    vec_change (@vec_change n v p x) q y = vec_change (vec_change v q y) p x.
-  Proof.
-    intros Hpq.
-    apply vec_pos_ext; intros r.
-    destruct (pos_eq_dec p r) as [?|Hpr].
-    + subst. rewrite (vec_change_neq _ _ (not_eq_sym Hpq)).
-      repeat rewrite vec_change_eq; auto.
-    + destruct (pos_eq_dec q r) as [?|Hqr].
-      * subst. rewrite (vec_change_neq _ _ Hpr).
-        repeat rewrite vec_change_eq; auto.
-      * repeat rewrite (vec_change_neq _ _ Hpr), (vec_change_neq _ _ Hqr); auto.
-  Qed.
-
   Variable eq_X_dec : forall x y : X, { x = y } + { x <> y }.
 
   Fixpoint vec_eq_dec n (u v : vec n) : { u = v } + { u <> v }.
@@ -578,6 +564,13 @@ Proof. auto. Qed.
 
 Fact vec_one_fst n : @vec_one (S n) pos0 = 1##vec_zero.
 Proof. apply vec_pos_ext; intros p; pos_inv p; rew vec. Qed.
+
+Lemma vec_change_comm {X} n v p q x y : p <> q ->
+vec_change (@vec_change X n v p x) q y = vec_change (vec_change v q y) p x.
+Proof.
+  intros Hpq. apply vec_pos_ext; intros r.
+  destruct (pos_eq_dec r p); destruct (pos_eq_dec r q); subst; now rew vec.
+Qed.
 
 Fact vec_one_nxt n p : @vec_one (S n) (pos_nxt p) = 0##vec_one p.
 Proof.
